backends/lean/Aeneas.lean
@@ -1,7 +1,6 @@
 import Aeneas.Arith
 import Aeneas.Bvify
 import Aeneas.BvTac
-import Aeneas.Diverge
 import Aeneas.FSimp
 import Aeneas.Int
 import Aeneas.List
