backends/lean/Aeneas/Std/Scalar/Core.lean
@@ -1,8 +1,6 @@
 import Lean
 import Lean.Meta.Tactic.Simp
 import Aeneas.Std.Core
-import Aeneas.Std.Core
-import Aeneas.Diverge.Core
 import Aeneas.Progress.Init
 import Aeneas.ScalarTac.ScalarTac
 import Aeneas.Bvify.Init
